pcuic/theories/PCUICArities.v
@@ -19,6 +19,31 @@ Implicit Types cf : checker_flags.
 
 Notation isWAT := (isWfArity typing).
 
+Lemma subslet_def {cf} {Σ : global_env_ext} {Γ Δ s na t T t'} : 
+  subslet Σ Γ s Δ ->
+  Σ;;; Γ |- subst0 s t : subst0 s T ->
+  t' = subst0 s t ->
+  subslet Σ Γ (t' :: s) (Δ ,, vdef na t T).
+Proof.
+  now intros sub Ht ->; constructor.
+Qed.
+
+Lemma subslet_ass_tip {cf} {Σ : global_env_ext} {Γ na t T} : 
+  Σ;;; Γ |- t : T ->
+  subslet Σ Γ [t] [vass na T].
+Proof.
+  intros; constructor. constructor.
+  all:now rewrite !subst_empty.
+Qed.
+
+Lemma subslet_def_tip {cf} {Σ : global_env_ext} {Γ na t T} : 
+  Σ;;; Γ |- t : T ->
+  subslet Σ Γ [t] [vdef na t T].
+Proof.
+  intros; apply subslet_def. constructor.
+  all:now rewrite !subst_empty.
+Qed.
+
 Lemma isType_Sort {cf:checker_flags} {Σ Γ s} :
   wf_universe Σ s ->
   wf_local Σ Γ ->
@@ -119,7 +144,7 @@ Proof.
 Qed.
 
 Lemma isType_tProd {cf:checker_flags} {Σ : global_env_ext} (HΣ' : wf Σ)
-      {Γ} (HΓ : wf_local Σ Γ) {na A B}
+      {Γ} {na A B}
   : isType Σ Γ (tProd na A B)
     <~> (isType Σ Γ A × isType Σ (Γ,, vass na A) B).
 Proof.
@@ -152,6 +177,26 @@ Proof.
   intros sub [s' Hs].
   exists s'. eapply (substitution _ _ Δ s _ _ _ HΣ' sub Hs).
 Qed.
+
+Lemma isType_wf_local {cf:checker_flags} {Σ Γ T} : isType Σ Γ T -> wf_local Σ Γ.
+Proof.
+  move=> [s Hs].
+  now eapply typing_wf_local.
+Qed.
+
+Lemma isType_apply {cf} {Σ : global_env_ext} {wfΣ : wf Σ} Γ na A B t : 
+  isType Σ Γ (tProd na A B) ->
+  Σ ;;; Γ |- t : A ->
+  isType Σ Γ (B {0 := t}).
+Proof.
+  move/isType_tProd => [hA hB] ht.
+  eapply (isType_subst _ (Δ:= [vass na A])); tea.
+  constructor; auto. pcuic.
+  now eapply subslet_ass_tip.
+Qed.
+
+Definition wf_typing_spine {cf} {Σ Γ T args T'} :=
+  isType Σ Γ T × typing_spine Σ Γ T args T'.
 
 Lemma typing_spine_letin_inv {cf:checker_flags} {Σ Γ na b B T args S} : 
   wf Σ.1 ->
@@ -307,12 +352,6 @@ Proof.
       simpl.   
       eapply IHΓ'; eauto.
       apply (type_mkProd_or_LetIn _ _ {| decl_body := None |}) => /=; eauto.
-Qed.
-
-Lemma isType_wf_local {cf:checker_flags} {Σ Γ T} : isType Σ Γ T -> wf_local Σ Γ.
-Proof.
-  move=> [s Hs].
-  now eapply typing_wf_local.
 Qed.
 
 Lemma app_context_push Γ Δ Δ' d : (Γ ,,, Δ ,,, Δ') ,, d = (Γ ,,, Δ ,,, (Δ' ,, d)).
