pcuic/theories/PCUICWeakeningEnv.v
@@ -555,13 +555,9 @@ Proof.
   - econstructor; eauto 2 with extends.
     now apply extends_wf_universe.
   - econstructor; eauto 2 with extends.
-    * eapply weakening_env_conv_ctx; eauto.
-      now destruct Σ.
     * revert X6. clear -Σ' wfΣ' extΣ.
       induction 1; constructor; eauto.
     * close_Forall. intros; intuition eauto with extends.
-      eapply weakening_env_conv_ctx; eauto.
-      now destruct Σ.
   - econstructor; eauto with extends.
     + eapply fix_guard_extends; eauto.
     + specialize (forall_Σ' _ wfΣ' extΣ).
